src/examples/Kuiper.ArrayView.Test1.fst
@@ -30,7 +30,6 @@ let base_view (et : Type) (len : nat) : aview et (lseq et len) = {
     len;
     sch = {
       ait      = natlt len;
-      ait_enum = solve;
     };
     step = {
       imap     = inj_id;
@@ -45,7 +44,6 @@ let r_base_view (et : Type) (len : nat) : aview et (lseq et len) = {
     len;
     sch = {
       ait      = natlt len;
-      ait_enum = solve;
     };
     step = {
       imap     = inj_nat_rev len;
@@ -169,6 +167,7 @@ fn write3
   requires p |-> s
   ensures  p |-> Seq.upd s 49 123ul
 {
+  IView.full_iff_cardinal (reverse_view u32 50).iview #_;
   varray_abs' (reverse_view u32 50) p;
   let a' = from_array (reverse_view u32 50) p;
   assert (pure (Seq.equal (to_seq (reverse_view u32 50) (from_seq (reverse_view u32 50) s)) s));
