src/lib/data/array/Kuiper.IArray.fst
@@ -106,14 +106,6 @@ fn iarray_ext
   fold iarray_pts_to a #f v2;
 }
 
-(* Note: the functions below use the Enumerable instance for vw.sch.ait
-   that is inside the aview record.
-   We do this since it's
-   not necessary for that enumeration to match the one in the typeclass system.
-   For example, for a matrix view, that enumeration can be anything
-   depending on the layout chosen, but the enumeration we want for the
-   **abstract indices** is just lexicographic. *)
-
 ghost
 fn iarray_explode
   (#et:Type)
@@ -299,7 +291,6 @@ fn iarray_reindex_
   (#et : Type0)
   (#vw : aiview)
   (#ait' : Type)
-  {| Enumerable.enumerable ait' |}
   (bij : vw.sch.ait =~ ait')
   (a : iarray et vw)
   (#f : perm)
@@ -326,7 +317,6 @@ fn iarray_reindex
   (#et : Type0)
   (#vw : aiview)
   (#ait' : Type)
-  {| Enumerable.enumerable ait' |}
   (bij : vw.sch.ait =~ ait')
   (a : iarray et vw)
   (#f : perm)
